Redesigned Basic.lean by redefining the Program type. Added new theorems. Old design will be archived in the Alternative.lean file.

Loop/Basic.lean
@@ -1,4 +1,10 @@
+/-
+Copyright: TODO
+Authors: Darío Silva Rodríguez
+-/
+
 import Mathlib.Data.Vector.Defs
+import Mathlib.Data.List.Basic
 
 /-!
 # The Loop programming language
@@ -11,35 +17,30 @@ Loop-computable is the same as primitive recursive.
 namespace Loop
 
 
-inductive Instruction where
-  | clear_var : Nat → Instruction
-  | increment_var : Nat → Instruction
-  | loop_var : Nat → List Instruction → Instruction
-open Instruction
-
+inductive Program where
+  | clear_var : Nat → Program
+  | increment_var : Nat → Program
+  | loop_var : Nat → Program → Program
+  | seq_execution : Program → Program → Program
+open Program
 
 notation "CLEAR X " n:68 => clear_var n
 notation "INC X " n:68 => increment_var n
-notation "LOOP X " n " DO " ls:68 => loop_var n ls
+notation "LOOP X " n " DO " ls " END" => loop_var n ls
 
-abbrev END : List Instruction := []
+instance : Append Program where
+  append p p' := seq_execution p p'
 
-
--- /- A Loop program is a list of instructions. -/
-def Program := List Instruction
-
--- example : Program := END
-
+example : Program := CLEAR X 0
 def example_1 : Program :=
-  LOOP X 1 DO (
-    LOOP X 2 DO (
-      INC X 0     ::
-    END)          ::
-  END)            ::
+  LOOP X 1 DO
+    INC X 0
+  END ++
+  LOOP X 2 DO
+    INC X 0
   END
 
-def VarState := List Nat
-
+abbrev VarState := List Nat
 
 def value_at (xs : VarState) (k : Nat) : Nat := xs.getD k 0
 
@@ -50,69 +51,188 @@ def clear_value (xs : VarState) (k : Nat) : VarState := xs.set k 0
 
 example : clear_value [3, 1, 5] 2 = [3, 1, 0] := rfl
 
-def inc_value (xs : VarState) (k : Nat) : VarState := xs.set k (value_at xs k + 1)
+def inc_value : VarState → Nat → VarState
+  | [],      0     => [1]
+  | [],      n + 1 => 0 :: inc_value [] n
+  | x :: xs, 0     => (x + 1) :: xs
+  | x :: xs, n + 1 => x :: inc_value xs n
 
 example : inc_value [3, 1, 5] 2 = [3, 1, 6] := by rfl
+-- example : inc_value [3, 1, 5] 4 = [3, 1, 5, 0, 1] := by rfl
 
 def init_state (v : Mathlib.Vector Nat n) : VarState := 0 :: v.toList
-
-mutual
-  def lines_of_code : Program → Nat
-    | [] => 0
-    | .clear_var _ :: tail => 1 + lines_of_code tail
-    | .increment_var _ :: tail => 1 + lines_of_code tail
-    | loop :: tail => lines_of_code_instruction loop + lines_of_code tail
-
-  def lines_of_code_instruction : Instruction → Nat
-    | .loop_var _ inner => 1 + lines_of_code inner
-    | _ => 1
-end
-
-attribute [local simp] lines_of_code lines_of_code_instruction
-
-example : lines_of_code example_1 = 3 := rfl
 
 def execution_from_state (xs : VarState) (p : Program) : VarState :=
   let rec loop_n_times : Nat → VarState → Program → VarState
   | 0, xs, _ => xs
   | n + 1, xs, p => loop_n_times n (execution_from_state xs p) p
-  termination_by n _ p => (lines_of_code p, n)
-
   match p with
-  | [] => xs
-  | .clear_var k      :: tail =>
-    execution_from_state (clear_value xs k) tail
-  | .increment_var k  :: tail =>
-    execution_from_state (inc_value xs k) tail
-  | .loop_var k inner :: tail =>
-    execution_from_state (loop_n_times (value_at xs k) xs inner) tail
-termination_by (lines_of_code p, 0)
+  | clear_var n => clear_value xs n
+  | increment_var n => inc_value xs n
+  | loop_var n p => loop_n_times (value_at xs n) xs p
+  | seq_execution p p' => execution_from_state (execution_from_state xs p) p'
 open execution_from_state
-
 
 def nary_program_function (p : Program) (n : Nat) (v : Mathlib.Vector Nat n) : Nat :=
   value_at (execution_from_state (init_state v) p) 0
 
 notation "⟦ " p " ⟧^(" n ") " => nary_program_function p n
 
-example : ⟦ example_1 ⟧^(2) ⟨[11, 11], rfl⟩ = 121 := by
-  simp [nary_program_function, init_state, example_1, execution_from_state, loop_n_times, value_at, inc_value, clear_value]
-
+example : ⟦ example_1 ⟧^(2) ⟨[23, 4], rfl⟩ = 27 := by
+  simp [nary_program_function, init_state, example_1, execution_from_state, loop_n_times, value_at, inc_value, clear_value, HAppend.hAppend, Append.append]
 
 def loop_computable (f : Mathlib.Vector Nat n → Nat) : Prop :=
   ∃ p : Program, ⟦ p ⟧^(n) = f
 
 -- -- -------
 def highest_var : Program → Nat
-  | [] => 0
-  | clear_var k :: tail =>
-    have : lines_of_code tail < lines_of_code (clear_var k :: tail) := by simp
-    max k (highest_var tail)
-  | increment_var k :: tail =>
-    have : lines_of_code tail < lines_of_code (increment_var k :: tail) := by simp
-    max k (highest_var tail)
-  | loop_var k inner :: tail =>
-    have : lines_of_code inner < lines_of_code (loop_var k inner :: tail) := by simp_arith
-    have : lines_of_code tail < lines_of_code (loop_var k inner :: tail) := by simp_arith
-    max k (max (highest_var inner) (highest_var tail))
-termination_by p => lines_of_code p
+  | clear_var n => n
+  | increment_var n => n
+  | loop_var n p => max n (highest_var p)
+  | seq_execution p p' => max (highest_var p) (highest_var p')
+
+abbrev List.zeros (n : Nat) : List Nat := List.replicate n 0
+
+-- /- A function is loop computable cleanly if it does not modify the initial state,. -/
+def loop_computable_cleanly (f : Mathlib.Vector Nat n → Nat) : Prop :=
+  ∃ p : Program, ∀ v : Mathlib.Vector Nat n,
+    execution_from_state (init_state v ++ List.zeros (highest_var p - n)) p
+    =
+    f v :: v.toList ++ List.zeros (highest_var p - n)
+
+theorem value_at_nil : value_at [] n = 0 := rfl
+theorem value_at_cons_zero : value_at (x :: xs) 0 = x := rfl
+theorem value_at_cons_succ : value_at (x :: xs) (n + 1) = value_at xs n := rfl
+
+theorem clear_value_nil : clear_value [] n = [] := rfl
+theorem clear_value_cons_zero : clear_value (x :: xs) 0 = 0 :: xs := rfl
+theorem clear_value_cons_succ : clear_value (x :: xs) (n + 1) = x :: clear_value xs n := rfl
+
+theorem inc_value_nil_zero : inc_value [] 0 = [1] := rfl
+theorem inc_value_nil_succ : inc_value [] (n + 1) = 0 :: inc_value [] n := rfl
+theorem inc_value_cons_zero : inc_value (x :: xs) 0 = (x + 1) :: xs := rfl
+theorem inc_value_cons_succ : inc_value (x :: xs) (n + 1) = x :: inc_value xs n := rfl
+
+
+theorem value_at_zeros_is_zero (n k : Nat) : value_at (List.zeros n) k = 0 := by
+  revert n
+  induction k
+  case zero =>
+    intro n
+    cases n <;> simp [value_at]
+  case succ ih =>
+    intro n
+    cases n
+    · simp [value_at]
+    · simp [List.replicate, value_at_cons_succ, ih]
+
+
+theorem append_zeros_does_not_change_value_at (xs : VarState) (n k : Nat) :
+    value_at xs k = value_at (xs ++ List.zeros n) k := by
+  revert k
+  induction xs
+  case nil => simp [value_at_nil, value_at_zeros_is_zero]
+  case cons head tail tail_ih =>
+    intro k
+    cases k
+    all_goals simp [value_at_cons_zero, value_at_cons_succ, tail_ih]
+
+theorem clear_value_clears_value (xs : VarState) :
+    value_at (clear_value xs n) k = if (n = k) then 0 else value_at xs k := by
+  revert n k
+  induction xs
+  case nil =>
+    simp [clear_value_nil, value_at_nil]
+  case cons x xs xs_ih =>
+    intro n k
+    cases n
+    · cases k <;> simp [clear_value, value_at]
+    · cases k
+      · simp [clear_value, value_at]
+      · simp [value_at_cons_succ]
+        exact xs_ih
+
+theorem inc_value_increments_value (xs : VarState) :
+    value_at (inc_value xs n) k = if (n = k) then value_at xs k + 1 else value_at xs k := by
+  revert n k
+  induction xs
+  case nil =>
+    intro n
+    induction n
+    case zero =>
+      simp [inc_value_nil_zero, value_at_nil]
+      intro k
+      cases k <;> simp [value_at]
+    case succ n n_ih =>
+      simp [inc_value, value_at_nil]
+      intro k
+      induction k
+
+      case zero =>
+        simp [value_at_cons_zero]
+      case succ k k_ih =>
+        simp [value_at_cons_succ]
+        simp [value_at_nil] at n_ih
+        exact n_ih
+
+  case cons x xs xs_ih =>
+    intro n
+    cases n
+    · simp [inc_value_cons_zero, value_at_cons_succ]
+      intro k
+      cases k <;> simp [value_at]
+    · simp [inc_value_cons_succ]
+      intro k
+      cases k <;> simp [value_at_cons_zero, value_at_cons_succ, xs_ih]
+
+
+theorem same_values_same_execution (p : Program) (xs ys : VarState) :
+    (∀ k : Nat, value_at xs k = value_at ys k) → ∀ k : Nat, value_at (execution_from_state xs p) k = value_at (execution_from_state ys p) k := by
+  revert xs ys
+  induction p
+  case clear_var n =>
+    intro xs ys h
+    simp [execution_from_state, clear_value_clears_value, h]
+  case increment_var n =>
+    intro xs ys h
+    simp [execution_from_state, inc_value_increments_value, h]
+  case loop_var n inner inner_ih =>
+    intro xs ys h
+    simp [execution_from_state, h]
+    generalize value_at ys n = x
+    revert xs ys
+    induction x
+    case zero =>
+      intro xs ys h
+      simp [loop_n_times, h]
+    case succ x x_ih =>
+      intro xs ys h
+      simp [loop_n_times]
+      apply x_ih (execution_from_state xs inner) (execution_from_state ys inner)
+      exact inner_ih xs ys h
+  case seq_execution p p' p_ih p'_ih =>
+    intro xs ys h
+    simp [execution_from_state]
+    apply p'_ih
+    apply p_ih
+    exact h
+
+theorem append_zeros_does_not_change_execution (n k : Nat) :
+    value_at (execution_from_state (xs ++ List.zeros n) p) k = value_at (execution_from_state xs p) k := by
+  have := append_zeros_does_not_change_value_at xs n
+  have := same_values_same_execution p xs (xs ++ List.zeros n) this k
+  exact this.symm
+
+theorem loop_computable_cleanly_is_loop_computable : loop_computable_cleanly f → loop_computable f := by
+  rename_i n
+  intro ⟨p, h⟩
+  exists p
+  apply funext
+  intro v
+  let dif := highest_var p - n
+  exact
+    calc
+      ⟦ p ⟧^(n) v = value_at (execution_from_state (init_state v) p) 0 := by rw [nary_program_function]
+                _ = value_at (execution_from_state (init_state v ++ List.zeros dif) p) 0 := by rw [append_zeros_does_not_change_execution ]
+                _ = value_at (f v :: v.toList ++ List.zeros dif) 0 := by rw [h v]
+                _ = f v := by rfl
