Loop/Alternative.lean
@@ -1,0 +1,195 @@
+import Mathlib.Data.Vector.Defs
+import Mathlib.Data.List.Basic
+
+/-!
+# The Loop programming language
+
+The goal of this file is to formally define the semantics of the Loop
+programming language, define what Loop-computable functions are, and prove that
+Loop-computable is the same as primitive recursive.
+-/
+
+namespace Loop
+
+
+inductive Instruction where
+  | clear_var : Nat → Instruction
+  | increment_var : Nat → Instruction
+  | loop_var : Nat → List Instruction → Instruction
+open Instruction
+
+
+notation "CLEAR X " n:68 => clear_var n
+notation "INC X " n:68 => increment_var n
+notation "LOOP X " n " DO " ls:68 => loop_var n ls
+
+abbrev END : List Instruction := []
+
+
+-- /- A Loop program is a list of instructions. -/
+def Program := List Instruction
+
+-- example : Program := END
+
+def example_1 : Program :=
+  LOOP X 1 DO (
+    LOOP X 2 DO (
+      INC X 0     ::
+    END)          ::
+  END)            ::
+  END
+
+abbrev VarState := List Nat
+
+
+def value_at (xs : VarState) (k : Nat) : Nat := xs.getD k 0
+
+example : value_at [3, 1, 5] 2 = 5 := rfl
+example : value_at [3, 1, 5] 7 = 0 := rfl
+
+def clear_value (xs : VarState) (k : Nat) : VarState := xs.set k 0
+
+example : clear_value [3, 1, 5] 2 = [3, 1, 0] := rfl
+
+def inc_value (xs : VarState) (k : Nat) : VarState := xs.set k (value_at xs k + 1)
+
+example : inc_value [3, 1, 5] 2 = [3, 1, 6] := by rfl
+
+def init_state (v : Mathlib.Vector Nat n) : VarState := 0 :: v.toList
+
+mutual
+  def lines_of_code : Program → Nat
+    | [] => 0
+    | .clear_var _ :: tail => 1 + lines_of_code tail
+    | .increment_var _ :: tail => 1 + lines_of_code tail
+    | loop :: tail => lines_of_code_instruction loop + lines_of_code tail
+
+  def lines_of_code_instruction : Instruction → Nat
+    | .loop_var _ inner => 1 + lines_of_code inner
+    | _ => 1
+end
+
+attribute [local simp] lines_of_code lines_of_code_instruction
+
+example : lines_of_code example_1 = 3 := rfl
+
+def execution_from_state (xs : VarState) (p : Program) : VarState :=
+  let rec loop_n_times : Nat → VarState → Program → VarState
+  | 0, xs, _ => xs
+  | n + 1, xs, p => loop_n_times n (execution_from_state xs p) p
+  termination_by n _ p => (lines_of_code p, n)
+
+  match p with
+  | [] => xs
+  | .clear_var k      :: tail =>
+    execution_from_state (clear_value xs k) tail
+  | .increment_var k  :: tail =>
+    execution_from_state (inc_value xs k) tail
+  | .loop_var k inner :: tail =>
+    execution_from_state (loop_n_times (value_at xs k) xs inner) tail
+termination_by (lines_of_code p, 0)
+open execution_from_state
+
+
+def nary_program_function (p : Program) (n : Nat) (v : Mathlib.Vector Nat n) : Nat :=
+  value_at (execution_from_state (init_state v) p) 0
+
+notation "⟦ " p " ⟧^(" n ") " => nary_program_function p n
+
+example : ⟦ example_1 ⟧^(2) ⟨[11, 11], rfl⟩ = 121 := by
+  simp [nary_program_function, init_state, example_1, execution_from_state, loop_n_times, value_at, inc_value, clear_value]
+
+
+def loop_computable (f : Mathlib.Vector Nat n → Nat) : Prop :=
+  ∃ p : Program, ⟦ p ⟧^(n) = f
+
+-- -- -------
+-- def highest_var : Program → Nat
+--   | [] => 0
+--   | clear_var k :: tail =>
+--     have : lines_of_code tail < lines_of_code (clear_var k :: tail) := by simp
+--     max k (highest_var tail)
+--   | increment_var k :: tail =>
+--     have : lines_of_code tail < lines_of_code (increment_var k :: tail) := by simp
+--     max k (highest_var tail)
+--   | loop_var k inner :: tail =>
+--     have : lines_of_code inner < lines_of_code (loop_var k inner :: tail) := by simp_arith
+--     have : lines_of_code tail < lines_of_code (loop_var k inner :: tail) := by simp_arith
+--     max k (max (highest_var inner) (highest_var tail))
+-- termination_by p => lines_of_code p
+
+-- abbrev List.zeros (n : Nat) : List Nat := List.replicate n 0
+
+-- -- /- A function is loop computable cleanly if it does not modify the initial state,. -/
+-- def loop_computable_cleanly (f : Mathlib.Vector Nat n → Nat) : Prop :=
+--   ∃ p : Program, ∀ v : Mathlib.Vector Nat n,
+--     execution_from_state (init_state v ++ List.zeros (highest_var p - n)) p
+--     =
+--     f v :: v.toList ++ List.zeros (highest_var p - n)
+
+-- theorem value_at_nil : value_at [] n = 0 := rfl
+-- theorem value_at_cons_zero : value_at (x :: xs) 0 = x := rfl
+-- theorem value_at_cons_succ : value_at (x :: xs) (n + 1) = value_at xs n := rfl
+
+-- theorem value_at_zeros_is_zero (n k : Nat) : value_at (List.zeros n) k = 0 := by
+--   revert n
+--   induction k
+--   case zero =>
+--     intro n
+--     cases n <;> simp [value_at]
+--   case succ ih =>
+--     intro n
+--     cases n
+--     · simp [value_at]
+--     · simp [List.replicate, value_at_cons_succ]
+--       apply ih
+
+-- theorem append_zeros_does_not_change_value_at (xs : VarState) (n k : Nat) :
+--     value_at xs k = value_at (xs ++ List.zeros n) k := by
+--   revert k
+--   induction xs
+--   case nil => simp [value_at_nil, value_at_zeros_is_zero]
+--   case cons head tail tail_ih =>
+--     intro k
+--     cases k
+--     all_goals simp [value_at_cons_zero, value_at_cons_succ]
+--     apply tail_ih
+
+
+-- theorem same_values_same_execution (p : Program) (xs ys : VarState) (k : Nat) :
+--     (∀ k : Nat, value_at xs k = value_at ys k) → value_at (execution_from_state xs p) k = value_at (execution_from_state ys p) k := by
+--   intro ih
+--   induction p
+--   case nil =>
+--     simp [execution_from_state, ih]
+--   case cons head tail tail_ih =>
+--     cases head
+--     all_goals simp [execution_from_state]
+--     ·
+--       sorry
+--     ·
+--       sorry
+--     ·
+--       sorry
+
+
+
+-- theorem append_zeros_does_not_change_execution (n k : Nat) :
+--     value_at (execution_from_state (xs ++ List.zeros n) p) k = value_at (execution_from_state xs p) k := by
+--   have := append_zeros_does_not_change_value_at xs n
+--   have := same_values_same_execution p xs (xs ++ List.zeros n) k this
+--   exact this.symm
+
+-- theorem loop_computable_cleanly_is_loop_computable : loop_computable_cleanly f → loop_computable f := by
+--   rename_i n
+--   intro ⟨p, h⟩
+--   exists p
+--   apply funext
+--   intro v
+--   let dif := highest_var p - n
+--   exact
+--     calc
+--       ⟦ p ⟧^(n) v = value_at (execution_from_state (init_state v) p) 0 := by rw [nary_program_function]
+--                 _ = value_at (execution_from_state (init_state v ++ List.zeros dif) p) 0 := by rw [append_zeros_does_not_change_execution ]
+--                 _ = value_at (f v :: v.toList ++ List.zeros dif) 0 := by rw [h v]
+--                 _ = f v := by rfl
